sha3_cmp_impl.v
@@ -50,5 +50,46 @@ Definition trivial_sha3_cmp (sstack_val_cmp: sstack_val_cmp_t) (soffset1 ssize1:
   false.
 
 
+Definition update_out_of_slot (u : memory_update sstack_val) (min max: N) (maxidx: nat) (sb: sbindings) (instk_height: nat) (ops: stack_op_instr_map) :=
+    match u with
+    | U_MSTORE _ offset _ =>
+        match follow_in_smap offset maxidx sb with
+        | Some (FollowSmapVal (SymBasicVal (Val v)) _ _) =>
+            orb ((wordToN v)+31 <? min)%N (max <? (wordToN v))%N
+        | _ => false
+        end
+    | U_MSTORE8 _ offset _ =>
+        match follow_in_smap offset maxidx sb with
+        | Some (FollowSmapVal (SymBasicVal (Val v)) _ _) =>
+            orb ((wordToN v) <? min)%N (max <? (wordToN v))%N
+        | _ => false
+        end
+    end.
+  
+Fixpoint remove_out_of_slot' (smem :smemory) (min max: N) (maxidx: nat) (sb: sbindings) (instk_height: nat) (ops: stack_op_instr_map) : smemory :=
+    match smem with
+    | [] => []
+    | u::us =>
+        if (update_out_of_slot u min max maxidx sb instk_height ops) 
+        then remove_out_of_slot' us min max maxidx sb instk_height ops
+        else u::(remove_out_of_slot' us min max maxidx sb instk_height ops)
+    end.
+
+Definition remove_out_of_slot (smem :smemory) (soffset ssize: sstack_val) (maxidx: nat) (sb: sbindings) (instk_height: nat) (ops: stack_op_instr_map) : smemory :=
+        match follow_in_smap soffset maxidx sb, follow_in_smap ssize maxidx sb with
+        | Some (FollowSmapVal (SymBasicVal (Val v1)) _ _), Some (FollowSmapVal (SymBasicVal (Val v2)) _ _) =>
+            remove_out_of_slot' smem (wordToN v1) ((wordToN v1)+(wordToN v2)-1)%N maxidx sb instk_height ops
+        | _, _ => smem
+        end. 
+
+Definition basic_sha3_cmp (sstack_val_cmp: sstack_val_cmp_t) (soffset1 ssize1: sstack_val) (smem1 :smemory) (soffset2 ssize2: sstack_val) (smem2 :smemory) (maxidx1: nat) (sb1: sbindings) (maxidx2: nat) (sb2: sbindings) (instk_height: nat) (ops: stack_op_instr_map) : bool :=
+  if (andb (sstack_val_cmp soffset1 soffset2 maxidx1 sb1 maxidx2 sb2 instk_height ops) (sstack_val_cmp ssize1 ssize2 maxidx1 sb1 maxidx2 sb2 instk_height ops)) then
+    let smem1 := remove_out_of_slot smem1 soffset1 ssize1 maxidx1 sb1 instk_height ops in
+    let smem2 := remove_out_of_slot smem2 soffset2 ssize2 maxidx2 sb2 instk_height ops in
+    po_memory_cmp sstack_val_cmp smem1 smem2 maxidx1 sb1 maxidx2 sb2 instk_height ops
+  else
+    false.
+
+
 
 End SHA3CmpImpl.
