sha3_cmp_impl_soundness.v
@@ -46,7 +46,7 @@ Import EvalCommon.
 Module SHA3CmpImplSoundness.
 
 
-  Theorem trivial_sha3_cmp_snd:
+  Lemma trivial_sha3_cmp_snd:
     safe_sha3_cmp_ext_wrt_sstack_value_cmp trivial_sha3_cmp.
   Proof.
     unfold safe_sha3_cmp_ext_wrt_sstack_value_cmp.
@@ -57,8 +57,9 @@ Module SHA3CmpImplSoundness.
     discriminate.
   Qed.
     
-  
-Definition trivial_sha3_cmp (sstack_val_cmp: sstack_val_cmp_t) (soffset1 ssize1: sstack_val) (smem1 :smemory) (soffset2 ssize2: sstack_val) (smem2 :smemory) (maxidx1: nat) (sb1: sbindings) (maxidx2: nat) (sb2: sbindings) (instk_height: nat) (ops: stack_op_instr_map) : bool :=
-  false.
+  Lemma basic_sha3_cmp_snd:
+    safe_sha3_cmp_ext_wrt_sstack_value_cmp basic_sha3_cmp.
+  Proof.
+    Admitted.
 
 End SHA3CmpImplSoundness.
