sstack_val_cmp_impl.v
@@ -40,77 +40,169 @@ Import SymbolicStateCmp.
 Require Import FORVES.eval_common.
 Import EvalCommon.
 
+Require Import FORVES.symbolic_state_dec.
+Import SymbolicStateDec.
+
 Module SStackValCmpImpl.
 
   Definition trivial_compare_sstack_val (smemory_cmp: smemory_cmp_ext_t) (sstorage_cmp: sstorage_cmp_ext_t) (sha3_cmp: sha3_cmp_ext_t) (d: nat) (sv1 sv2: sstack_val) (maxidx1: nat) (sb1: sbindings) (maxidx2: nat) (sb2: sbindings) (instk_height: nat) (ops: stack_op_instr_map) : bool :=
-    false.
-
-Fixpoint basic_compare_sstack_val (smemory_cmp: smemory_cmp_ext_t) (sstorage_cmp: sstorage_cmp_ext_t) (sha3_cmp: sha3_cmp_ext_t) (d: nat) (sv1 sv2: sstack_val) (maxidx1: nat) (sb1: sbindings) (maxidx2: nat) (sb2: sbindings) (instk_height: nat) (ops: stack_op_instr_map) : bool :=
-  match d with
-  | 0 => false
-  | S d' =>
-      let basic_compare_sstack_val_rec :=
-        basic_compare_sstack_val smemory_cmp sstorage_cmp sha3_cmp d' in
-      match follow_in_smap sv1 maxidx1 sb1 with
-      | None => false
-      | Some (FollowSmapVal smv1 maxidx1' sb1') =>
-          match  follow_in_smap sv2 maxidx2 sb2 with
-          | None => false
-          | Some (FollowSmapVal smv2 maxidx2' sb2') =>
-              match smv1, smv2 with 
-              | SymBasicVal sv1', SymBasicVal sv2' =>
-                  match sv1',sv2' with
-                  | Val w1, Val w2 => weqb w1 w2
-                  | InStackVar n1, InStackVar n2 => (andb (n1 =? n2) (andb (n1 <? instk_height) (n2 <? instk_height)))
-                  | _, _ => false
-                  end
-              | SymMETAPUSH cat1 v1, SymMETAPUSH cat2 v2 => andb (cat1 =? cat2)%N (v1 =? v2)%N
-              | SymOp label1 args1, SymOp label2 args2 =>
-                  if label1 =?i label2 then
-                    match ops label1 with
-                      OpImp _ _ H_Comm _ =>
-                        match (fold_right_two_lists (fun e1 e2 => basic_compare_sstack_val_rec e1 e2 maxidx1' sb1' maxidx2' sb2' instk_height ops) args1 args2) with
-                        | true => true
-                        | false =>
-                            match H_Comm with
-                            | Some comm_proof =>
-                                match args1, args2 with
-                                | [a1;a2],[b1;b2] =>
-                                    if basic_compare_sstack_val_rec a1 b2 maxidx1' sb1' maxidx2' sb2' instk_height ops
-                                    then basic_compare_sstack_val_rec a2 b1 maxidx1' sb1' maxidx2' sb2' instk_height ops
-                                    else false
-                                | _, _ => false
-                                end
-                            | None => false
-                            end
-                        end
+    match d with
+    | 0 => false
+    | S d' =>
+        match sv1,sv2 with
+        | Val w1, Val w2 => weqb w1 w2
+        | InStackVar n1, InStackVar n2 => (andb (n1 =? n2) (andb (n1 <? instk_height) (n2 <? instk_height)))
+        | FreshVar n1, FreshVar n2 =>
+            if (n1 =? n2)
+            then if (maxidx1 =? maxidx2)
+                 then if (sbindings_eq_dec sb1 sb2)
+                      then true
+                      else false
+                 else false
+            else false
+        | _, _ => false
+        end
+    end.
+  
+  
+  Fixpoint basic_compare_sstack_val (smemory_cmp: smemory_cmp_ext_t) (sstorage_cmp: sstorage_cmp_ext_t) (sha3_cmp: sha3_cmp_ext_t) (d: nat) (sv1 sv2: sstack_val) (maxidx1: nat) (sb1: sbindings) (maxidx2: nat) (sb2: sbindings) (instk_height: nat) (ops: stack_op_instr_map) : bool :=
+    match d with
+    | 0 => false
+    | S d' =>
+        let basic_compare_sstack_val_rec :=
+          basic_compare_sstack_val smemory_cmp sstorage_cmp sha3_cmp d' in
+        match follow_in_smap sv1 maxidx1 sb1 with
+        | None => false
+        | Some (FollowSmapVal smv1 maxidx1' sb1') =>
+            match  follow_in_smap sv2 maxidx2 sb2 with
+            | None => false
+            | Some (FollowSmapVal smv2 maxidx2' sb2') =>
+                match smv1, smv2 with 
+                | SymBasicVal sv1', SymBasicVal sv2' =>
+                    match sv1',sv2' with
+                    | Val w1, Val w2 => weqb w1 w2
+                    | InStackVar n1, InStackVar n2 => (andb (n1 =? n2) (andb (n1 <? instk_height) (n2 <? instk_height)))
+                    | _, _ => false
                     end
-                  else false
-              | SymMLOAD soffset1 smem1, SymMLOAD soffset2 smem2 =>
-                  if basic_compare_sstack_val smemory_cmp sstorage_cmp sha3_cmp d' soffset1 soffset2 maxidx1' sb1' maxidx2' sb2' instk_height ops
-                  then smemory_cmp basic_compare_sstack_val_rec smem1 smem2 maxidx1' sb1' maxidx2' sb2' instk_height ops
-                  else false
-              | SymSLOAD skey1 sstrg1, SymSLOAD skey2 sstrg2 => 
-                  if basic_compare_sstack_val smemory_cmp sstorage_cmp sha3_cmp d' skey1 skey2 maxidx1' sb1' maxidx2' sb2' instk_height ops
-                  then sstorage_cmp basic_compare_sstack_val_rec sstrg1 sstrg2 maxidx1' sb1' maxidx2' sb2' instk_height ops
-                  else false
-              | SymSHA3 soffset1 ssize1 smem1, SymSHA3 soffset2 ssize2 smem2 =>
-                  (* the nested if is to avoid using band *)
-                  if (if basic_compare_sstack_val_rec soffset1 soffset2 maxidx1' sb1' maxidx2' sb2' instk_height ops then
-                        if basic_compare_sstack_val_rec ssize1 ssize2 maxidx1' sb1' maxidx2' sb2' instk_height ops then
-                           smemory_cmp basic_compare_sstack_val_rec smem1 smem2 maxidx1' sb1' maxidx2' sb2' instk_height ops 
+                | SymMETAPUSH cat1 v1, SymMETAPUSH cat2 v2 => andb (cat1 =? cat2)%N (v1 =? v2)%N
+                | SymOp label1 args1, SymOp label2 args2 =>
+                    if label1 =?i label2 then
+                      match ops label1 with
+                        OpImp _ _ H_Comm _ =>
+                          match (fold_right_two_lists (fun e1 e2 => basic_compare_sstack_val_rec e1 e2 maxidx1' sb1' maxidx2' sb2' instk_height ops) args1 args2) with
+                          | true => true
+                          | false =>
+                              match H_Comm with
+                              | Some comm_proof =>
+                                  match args1, args2 with
+                                  | [a1;a2],[b1;b2] =>
+                                      if basic_compare_sstack_val_rec a1 b2 maxidx1' sb1' maxidx2' sb2' instk_height ops
+                                      then basic_compare_sstack_val_rec a2 b1 maxidx1' sb1' maxidx2' sb2' instk_height ops
+                                      else false
+                                  | _, _ => false
+                                  end
+                              | None => false
+                              end
+                          end
+                      end
+                    else false
+                | SymMLOAD soffset1 smem1, SymMLOAD soffset2 smem2 =>
+                    if basic_compare_sstack_val smemory_cmp sstorage_cmp sha3_cmp d' soffset1 soffset2 maxidx1' sb1' maxidx2' sb2' instk_height ops
+                    then smemory_cmp basic_compare_sstack_val_rec smem1 smem2 maxidx1' sb1' maxidx2' sb2' instk_height ops
+                    else false
+                | SymSLOAD skey1 sstrg1, SymSLOAD skey2 sstrg2 => 
+                    if basic_compare_sstack_val smemory_cmp sstorage_cmp sha3_cmp d' skey1 skey2 maxidx1' sb1' maxidx2' sb2' instk_height ops
+                    then sstorage_cmp basic_compare_sstack_val_rec sstrg1 sstrg2 maxidx1' sb1' maxidx2' sb2' instk_height ops
+                    else false
+                | SymSHA3 soffset1 ssize1 smem1, SymSHA3 soffset2 ssize2 smem2 =>
+                    (* the nested if is to avoid using band *)
+                    if (if basic_compare_sstack_val_rec soffset1 soffset2 maxidx1' sb1' maxidx2' sb2' instk_height ops then
+                          if basic_compare_sstack_val_rec ssize1 ssize2 maxidx1' sb1' maxidx2' sb2' instk_height ops then
+                            smemory_cmp basic_compare_sstack_val_rec smem1 smem2 maxidx1' sb1' maxidx2' sb2' instk_height ops 
+                          else
+                            false
                         else
-                          false
-                      else
-                        false)
-                  then true
-                  else 
-                    sha3_cmp basic_compare_sstack_val_rec soffset1 ssize1 smem1 soffset2 ssize2 smem2 maxidx1' sb1' maxidx2' sb2' instk_height ops
-              | _, _ => false
-              end
-          end
-      end
-  end.
+                          false)
+                    then true
+                    else 
+                      sha3_cmp basic_compare_sstack_val_rec soffset1 ssize1 smem1 soffset2 ssize2 smem2 maxidx1' sb1' maxidx2' sb2' instk_height ops
+                | _, _ => false
+                end
+            end
+        end
+    end.
+
+
+
+  Fixpoint basic_compare_sstack_val_w_eq_chk (smemory_cmp: smemory_cmp_ext_t) (sstorage_cmp: sstorage_cmp_ext_t) (sha3_cmp: sha3_cmp_ext_t) (d: nat) (sv1 sv2: sstack_val) (maxidx1: nat) (sb1: sbindings) (maxidx2: nat) (sb2: sbindings) (instk_height: nat) (ops: stack_op_instr_map) : bool :=
+    if (trivial_compare_sstack_val smemory_cmp sstorage_cmp sha3_cmp d sv1 sv2 maxidx1 sb1 maxidx2 sb2 instk_height ops)
+    then true
+    else
+    match d with
+    | 0 => false
+    | S d' =>
+        let basic_compare_sstack_val_w_eq_chk_rec :=
+          basic_compare_sstack_val_w_eq_chk smemory_cmp sstorage_cmp sha3_cmp d' in
+        match follow_in_smap sv1 maxidx1 sb1 with
+        | None => false
+        | Some (FollowSmapVal smv1 maxidx1' sb1') =>
+            match  follow_in_smap sv2 maxidx2 sb2 with
+            | None => false
+            | Some (FollowSmapVal smv2 maxidx2' sb2') =>
+                match smv1, smv2 with 
+                | SymBasicVal sv1', SymBasicVal sv2' =>
+                    match sv1',sv2' with
+                    | Val w1, Val w2 => weqb w1 w2
+                    | InStackVar n1, InStackVar n2 => (andb (n1 =? n2) (andb (n1 <? instk_height) (n2 <? instk_height)))
+                    | _, _ => false
+                    end
+                | SymMETAPUSH cat1 v1, SymMETAPUSH cat2 v2 => andb (cat1 =? cat2)%N (v1 =? v2)%N
+                | SymOp label1 args1, SymOp label2 args2 =>
+                    if label1 =?i label2 then
+                      match ops label1 with
+                        OpImp _ _ H_Comm _ =>
+                          match (fold_right_two_lists (fun e1 e2 => basic_compare_sstack_val_w_eq_chk_rec e1 e2 maxidx1' sb1' maxidx2' sb2' instk_height ops) args1 args2) with
+                          | true => true
+                          | false =>
+                              match H_Comm with
+                              | Some comm_proof =>
+                                  match args1, args2 with
+                                  | [a1;a2],[b1;b2] =>
+                                      if basic_compare_sstack_val_w_eq_chk_rec a1 b2 maxidx1' sb1' maxidx2' sb2' instk_height ops
+                                      then basic_compare_sstack_val_w_eq_chk_rec a2 b1 maxidx1' sb1' maxidx2' sb2' instk_height ops
+                                      else false
+                                  | _, _ => false
+                                  end
+                              | None => false
+                              end
+                          end
+                      end
+                    else false
+                | SymMLOAD soffset1 smem1, SymMLOAD soffset2 smem2 =>
+                    if basic_compare_sstack_val_w_eq_chk smemory_cmp sstorage_cmp sha3_cmp d' soffset1 soffset2 maxidx1' sb1' maxidx2' sb2' instk_height ops
+                    then smemory_cmp basic_compare_sstack_val_w_eq_chk_rec smem1 smem2 maxidx1' sb1' maxidx2' sb2' instk_height ops
+                    else false
+                | SymSLOAD skey1 sstrg1, SymSLOAD skey2 sstrg2 => 
+                    if basic_compare_sstack_val_w_eq_chk smemory_cmp sstorage_cmp sha3_cmp d' skey1 skey2 maxidx1' sb1' maxidx2' sb2' instk_height ops
+                    then sstorage_cmp basic_compare_sstack_val_w_eq_chk_rec sstrg1 sstrg2 maxidx1' sb1' maxidx2' sb2' instk_height ops
+                    else false
+                | SymSHA3 soffset1 ssize1 smem1, SymSHA3 soffset2 ssize2 smem2 =>
+                    (* the nested if is to avoid using band *)
+                    if (if basic_compare_sstack_val_w_eq_chk_rec soffset1 soffset2 maxidx1' sb1' maxidx2' sb2' instk_height ops then
+                          if basic_compare_sstack_val_w_eq_chk_rec ssize1 ssize2 maxidx1' sb1' maxidx2' sb2' instk_height ops then
+                            smemory_cmp basic_compare_sstack_val_w_eq_chk_rec smem1 smem2 maxidx1' sb1' maxidx2' sb2' instk_height ops 
+                          else
+                            false
+                        else
+                          false)
+                    then true
+                    else 
+                      sha3_cmp basic_compare_sstack_val_w_eq_chk_rec soffset1 ssize1 smem1 soffset2 ssize2 smem2 maxidx1' sb1' maxidx2' sb2' instk_height ops
+                | _, _ => false
+                end
+            end
+        end
+    end.
 
 
 
