extract_ocaml.v
@@ -19,7 +19,7 @@
     - Extract option
     - Extract nat into an efficient type.
     - Extract bbv library Word into an efficient type. *)
- 
+  
 From Coq Require Import Strings.String.
 Require Import List.
 Import ListNotations.
@@ -32,6 +32,33 @@ Import ExtrOcamlString.
 Extract Inductive bool => "bool" [ "true" "false" ].
 Extract Inductive list => "list" [ "[]" "(::)" ].
 Extract Inductive prod => "( * )" [ "( , )" ].
+Extract Inductive sumbool => "bool" ["true" "false"].
+
+(*
+Extract Inductive nat => int [ "0" "Stdlib.Int.succ" ]
+ "(fun fO fS n -> if n=0 then fO () else fS (n-1))".
+
+
+Extract Constant plus => "(+)".
+Extract Constant pred => "fun n -> Stdlib.max 0 (n-1)".
+Extract Constant minus => "fun n m -> Stdlib.max 0 (n-m)".
+Extract Constant mult => "( * )".
+Extract Inlined Constant max => "Stdlib.max".
+Extract Inlined Constant min => "Stdlib.min".
+Extract Inlined Constant Nat.eqb => "(=)".
+Extract Inlined Constant EqNat.eq_nat_decide => "(=)".
+
+Extract Inlined Constant Peano_dec.eq_nat_dec => "(=)".
+
+Extract Constant Nat.compare =>
+ "fun n m -> if n=m then Eq else if n<m then Lt else Gt".
+Extract Inlined Constant Compare_dec.leb => "(<=)".
+Extract Inlined Constant Compare_dec.le_lt_dec => "(<=)".
+Extract Inlined Constant Compare_dec.lt_dec => "(<)".
+Extract Constant Compare_dec.lt_eq_lt_dec =>
+ "fun n m -> if n>m then None else Some (n<m)".
+
+*)
 
 (** Program Extractions **)
 (*  Examples from example.v are extracted and directly tested.
