sstack_val_cmp_impl_soundness.v
@@ -36,6 +36,9 @@ Import ValidSymbolicState.
 Require Import FORVES.valid_symbolic_state.
 Import ValidSymbolicState.
 
+Require Import FORVES.symbolic_execution_soundness.
+Import SymbolicExecutionSoundness.
+
 Require Import FORVES.symbolic_state_cmp.
 Import SymbolicStateCmp.
 
@@ -45,6 +48,8 @@ Import SStackValCmpImpl.
 Require Import FORVES.eval_common.
 Import EvalCommon.
 
+Require Import FORVES.symbolic_state_dec.
+Import SymbolicStateDec.
 
 Module SStackValCmpImplSoundness.
 
@@ -62,14 +67,71 @@ Module SStackValCmpImplSoundness.
     safe_sstack_value_cmp_wrt_others trivial_compare_sstack_val.
   Proof.
     unfold safe_sstack_value_cmp_wrt_others.
-    intros.
+    intros d smemory_cmp sstorage_cmp sha3_cmp.
     unfold safe_sstack_val_cmp_ext_2_d.
     unfold safe_sstack_val_cmp_ext_1_d.
-    intros.
+    intros H_safe_smemory_cmp H_safe_sstorage_cmp H_safe_sha3_cmp.
+    intros d' H_d'_le_Sd'.
     unfold safe_sstack_val_cmp.
-    unfold trivial_compare_sstack_val.
-    intros.
-    discriminate.
+    intros sv1 sv2 maxidx1 bs1 maxidx2 bs2 instk_height ops H_valid_sv1 H_valid_sv2 H_valid_bs1 H_valid_bs2 H_cmp.
+    intros stk mem strg ctx H_stk_len.
+    unfold trivial_compare_sstack_val in H_cmp.
+    destruct d' as [|d''] eqn:E_d; try discriminate.
+
+    unfold eval_sstack_val.
+
+    destruct sv1 as [w1 | n1 | n1]; destruct sv2 as [w2 | n2 | n2] eqn:E_sv2; try discriminate.
+
+    + apply weqb_sound in H_cmp.
+
+      pose proof (eval_sstack_val'_Val w1 stk mem strg ctx maxidx1 bs1 ops) as H_eval_w1.
+      pose proof (eval_sstack_val'_Val w2 stk mem strg ctx maxidx2 bs2 ops) as H_eval_w2.
+      rewrite H_eval_w1.
+      rewrite H_eval_w2.
+      rewrite H_cmp.
+      exists w2.
+      split; reflexivity.
+
+    + pose proof (eval_sstack_val'_InStackVar n1 stk mem strg ctx maxidx1 bs1 ops) as H_eval_instkv_n1.
+      pose proof (eval_sstack_val'_InStackVar n2 stk mem strg ctx maxidx2 bs2 ops) as H_eval_instkv_n2.
+      rewrite H_eval_instkv_n1.
+      rewrite H_eval_instkv_n2.
+
+      apply andb_prop in H_cmp.
+      destruct H_cmp as [H_cmp_1 H_cmp].
+      apply andb_prop in H_cmp.
+      destruct H_cmp as [H_cmp_2 H_cmp_3].
+      
+      apply Nat.eqb_eq in H_cmp_1.
+      apply Nat.ltb_lt in H_cmp_2.
+      apply Nat.ltb_lt in H_cmp_3.
+
+      rewrite <- H_stk_len in H_cmp_3.
+      
+      pose proof (nth_error_ok' EVMWord stk n2 H_cmp_3) as H_nth_error_ok'.
+      destruct  H_nth_error_ok' as [v'  H_nth_error_ok'].
+      
+      rewrite H_cmp_1.
+      rewrite H_nth_error_ok'.
+      exists v'.
+      split; try reflexivity.
+      
+    + destruct (n1 =? n2) eqn:E_n1_eq_n2; try discriminate.
+      destruct (maxidx1 =? maxidx2) eqn:E_maxidx1_eq_maxidx2; try discriminate.
+      destruct (sbindings_eq_dec bs1 bs2) eqn:E_bs1_eq_bs2; try discriminate.
+      apply Nat.eqb_eq in E_n1_eq_n2.
+      apply Nat.eqb_eq in E_maxidx1_eq_maxidx2.
+
+      rewrite E_n1_eq_n2.
+      rewrite E_maxidx1_eq_maxidx2.
+      rewrite e.
+                  
+      pose proof (eval_sstack_val'_succ (S maxidx2) instk_height (FreshVar n2) stk mem strg ctx maxidx2 bs2 ops (eq_sym H_stk_len) H_valid_sv2 H_valid_bs2 (gt_Sn_n maxidx2)) as H_eval_sv2.
+      destruct H_eval_sv2 as [v2 H_eval_sv2].
+
+      rewrite H_eval_sv2.
+      exists v2.
+      split; try reflexivity.
   Qed.
     
 
@@ -85,7 +147,7 @@ Module SStackValCmpImplSoundness.
 
   Lemma basic_compare_sstack_val_snd:
     safe_sstack_value_cmp_wrt_others basic_compare_sstack_val.
-  Proof.
+  Proof.  
     unfold safe_sstack_value_cmp_wrt_others.
     induction d as [|d' IHd'].
     - intros smemory_cmp sstorage_cmp sha3_cmp H_safe_smemory_cmp H_safe_sstorage_cmp H_safe_sha3_cmp.
@@ -94,7 +156,7 @@ Module SStackValCmpImplSoundness.
       intros d' H_d'_le_1.
       unfold safe_sstack_val_cmp.
       intros sv1 sv2 maxidx1 sb1 maxidx2 sb2 instk_height ops H_valid_sv1 H_valid_sv2 H_valid_sb1 H_valid_sb2 H_cmp_sv1_sv2.      apply Nat.leb_le in H_d'_le_1 as H_d'_le_1_leb.
-
+ 
       intros stk mem strg ctx H_len_stk.
       unfold eval_sstack_val.
       unfold eval_sstack_val'. fold eval_sstack_val'.
@@ -112,13 +174,16 @@ Module SStackValCmpImplSoundness.
 
       rewrite H_follow_suc_sv1 in H_cmp_sv1_sv2.
       rewrite H_follow_suc_sv2 in H_cmp_sv1_sv2.
-
+ 
       pose proof (valid_follow_in_smap sb1 sv1 instk_height maxidx1 ops smv1 maxidx1' sb1' H_valid_sv1 H_valid_sb1 H_follow_suc_sv1) as H_follow_valid_sv1.
       pose proof (valid_follow_in_smap sb2 sv2 instk_height maxidx2 ops smv2 maxidx2' sb2' H_valid_sv2 H_valid_sb2 H_follow_suc_sv2) as H_follow_valid_sv2.
 
+      
       destruct smv1 eqn:E_smv1; destruct smv2 eqn:E_smv2; try discriminate.
 
-      + destruct val; destruct val0; try discriminate.
+      + 
+
+        destruct val; destruct val0; try discriminate.
         * apply weqb_sound in H_cmp_sv1_sv2.
           rewrite H_cmp_sv1_sv2.
           exists val0.
@@ -689,5 +754,773 @@ Module SStackValCmpImplSoundness.
         split; reflexivity.          
   Qed.
 
+  Lemma basic_compare_sstack_val_w_eq_chk_d0_snd:
+    sstack_val_cmp_fail_for_d_eq_0 basic_compare_sstack_val_w_eq_chk.
+  Proof.
+    unfold sstack_val_cmp_fail_for_d_eq_0.
+    intros.
+    simpl.
+    reflexivity.
+  Qed.
+
+  Lemma basic_compare_sstack_val_w_eq_chk_snd:
+    safe_sstack_value_cmp_wrt_others basic_compare_sstack_val_w_eq_chk.
+  Proof.
+    unfold safe_sstack_value_cmp_wrt_others.
+    induction d as [|d' IHd'].
+    - intros smemory_cmp sstorage_cmp sha3_cmp H_safe_smemory_cmp H_safe_sstorage_cmp H_safe_sha3_cmp.
+      unfold safe_sstack_val_cmp_ext_2_d.
+      unfold safe_sstack_val_cmp_ext_1_d.
+      intros d' H_d'_le_1.
+      unfold safe_sstack_val_cmp.
+      intros sv1 sv2 maxidx1 sb1 maxidx2 sb2 instk_height ops H_valid_sv1 H_valid_sv2 H_valid_sb1 H_valid_sb2 H_cmp_sv1_sv2.      apply Nat.leb_le in H_d'_le_1 as H_d'_le_1_leb.
+
+ 
+      destruct d' as [|d''] eqn:E_d'; try discriminate; destruct d'' as [|d'''] eqn:E_d''; try discriminate.
+      unfold basic_compare_sstack_val_w_eq_chk in H_cmp_sv1_sv2.
+
+      intros stk mem strg ctx H_len_stk.
+      unfold eval_sstack_val.
+
+      destruct(trivial_compare_sstack_val smemory_cmp sstorage_cmp sha3_cmp 1 sv1 sv2 maxidx1 sb1 maxidx2 sb2 instk_height ops) eqn:E_trivial_chk.
+
+      (* when calling trivial check *)
+      unfold trivial_compare_sstack_val in E_trivial_chk.
+      destruct sv1 as [w1 | n1 | n1]; destruct sv2 as [w2 | n2 | n2] eqn:E_sv2; try discriminate.
+
+        (* Val *)
+        apply weqb_sound in E_trivial_chk.
+
+        pose proof (eval_sstack_val'_Val w1 stk mem strg ctx maxidx1 sb1 ops) as H_eval_w1.
+        pose proof (eval_sstack_val'_Val w2 stk mem strg ctx maxidx2 sb2 ops) as H_eval_w2.
+        rewrite H_eval_w1.
+        rewrite H_eval_w2.
+        rewrite E_trivial_chk.
+        exists w2.
+        split; reflexivity.
+
+        (* InStackVar *)
+        pose proof (eval_sstack_val'_InStackVar n1 stk mem strg ctx maxidx1 sb1 ops) as H_eval_instkv_n1.
+        pose proof (eval_sstack_val'_InStackVar n2 stk mem strg ctx maxidx2 sb2 ops) as H_eval_instkv_n2.
+        rewrite H_eval_instkv_n1.
+        rewrite H_eval_instkv_n2.
+
+        apply andb_prop in E_trivial_chk.
+        destruct E_trivial_chk as [E_trivial_chk_1 E_trivial_chk].
+        apply andb_prop in E_trivial_chk.
+        destruct E_trivial_chk as [E_trivial_chk_2 E_trivial_chk_3].
+        
+        apply Nat.eqb_eq in E_trivial_chk_1.
+        apply Nat.ltb_lt in E_trivial_chk_2.
+        apply Nat.ltb_lt in E_trivial_chk_3.
+
+        rewrite <- H_len_stk in E_trivial_chk_3.
+        
+        pose proof (nth_error_ok' EVMWord stk n2 E_trivial_chk_3) as H_nth_error_ok'.
+        destruct  H_nth_error_ok' as [v'  H_nth_error_ok'].
+        
+        rewrite E_trivial_chk_1.
+        rewrite H_nth_error_ok'.
+        exists v'.
+        split; try reflexivity.
+        
+        (* FreshVar *)
+        destruct (n1 =? n2) eqn:E_n1_eq_n2; try discriminate.
+        destruct (maxidx1 =? maxidx2) eqn:E_maxidx1_eq_maxidx2; try discriminate.
+        destruct (sbindings_eq_dec sb1 sb2) eqn:E_bs1_eq_bs2; try discriminate.
+        apply Nat.eqb_eq in E_n1_eq_n2.
+        apply Nat.eqb_eq in E_maxidx1_eq_maxidx2.
+
+        rewrite E_n1_eq_n2.
+        rewrite E_maxidx1_eq_maxidx2.
+        rewrite e.
+                  
+        pose proof (eval_sstack_val'_succ (S maxidx2) instk_height (FreshVar n2) stk mem strg ctx maxidx2 sb2 ops (eq_sym H_len_stk) H_valid_sv2 H_valid_sb2 (gt_Sn_n maxidx2)) as H_eval_sv2.
+        destruct H_eval_sv2 as [v2 H_eval_sv2].
+
+        rewrite H_eval_sv2.
+        exists v2.
+        split; try reflexivity.
+      (* end of call to trivial chk *)
+
+      unfold eval_sstack_val'. fold eval_sstack_val'.
+
+      unfold basic_compare_sstack_val_w_eq_chk in H_cmp_sv1_sv2.
+      
+      pose proof (follow_in_smap_suc sb1 sv1 instk_height maxidx1 ops H_valid_sv1 H_valid_sb1) as H_follow_suc_sv1.
+      destruct H_follow_suc_sv1 as [smv1 [maxidx1' [sb1' [H_follow_suc_sv1 _]]]].
+      pose proof (follow_in_smap_suc sb2 sv2 instk_height maxidx2 ops H_valid_sv2 H_valid_sb2) as H_follow_suc_sv2.
+      destruct H_follow_suc_sv2 as [smv2 [maxidx2' [sb2' [H_follow_suc_sv2 _]]]].
+
+      rewrite H_follow_suc_sv1.
+      rewrite H_follow_suc_sv2.
+
+      rewrite H_follow_suc_sv1 in H_cmp_sv1_sv2.
+      rewrite H_follow_suc_sv2 in H_cmp_sv1_sv2.
+ 
+      pose proof (valid_follow_in_smap sb1 sv1 instk_height maxidx1 ops smv1 maxidx1' sb1' H_valid_sv1 H_valid_sb1 H_follow_suc_sv1) as H_follow_valid_sv1.
+      pose proof (valid_follow_in_smap sb2 sv2 instk_height maxidx2 ops smv2 maxidx2' sb2' H_valid_sv2 H_valid_sb2 H_follow_suc_sv2) as H_follow_valid_sv2.
+
+      
+      destruct smv1 eqn:E_smv1; destruct smv2 eqn:E_smv2; try discriminate.
+
+      + 
+
+        destruct val; destruct val0; try discriminate.
+        * apply weqb_sound in H_cmp_sv1_sv2.
+          rewrite H_cmp_sv1_sv2.
+          exists val0.
+          split; reflexivity.
+        * apply andb_prop in H_cmp_sv1_sv2 as [H_var_va0 H_cmp_sv1_sv2].
+          apply andb_prop in H_cmp_sv1_sv2 as [H_var_lt_inskt H_var0_lt_instk].
+          apply Nat.eqb_eq in H_var_va0.
+          rewrite H_var_va0.
+          rewrite <- H_len_stk in H_var0_lt_instk.
+          apply Nat.ltb_lt in H_var0_lt_instk.
+          pose proof (nth_error_nth' stk WZero H_var0_lt_instk) as H_nth_error.
+          rewrite H_nth_error.
+          exists (nth var0 stk WZero).
+          split; reflexivity.
+      + apply andb_prop in H_cmp_sv1_sv2 as [ H_cmp_sv1_sv2_0  H_cmp_sv1_sv2_1].
+        apply N.eqb_eq in H_cmp_sv1_sv2_0.
+        apply N.eqb_eq in H_cmp_sv1_sv2_1.
+        rewrite H_cmp_sv1_sv2_0.
+        rewrite H_cmp_sv1_sv2_1.
+        exists (get_tags_ctx ctx cat0 val0). split; reflexivity.
+      + destruct (label =?i label0) eqn:E_eqb_label_label0; try discriminate.
+        apply eqb_stack_op_instr_eq in E_eqb_label_label0 as E_eq_label_label0.
+        rewrite <- E_eq_label_label0.
+        rewrite <- E_eq_label_label0 in H_follow_suc_sv2.
+        destruct (ops label) eqn:E_ops_label.
+        destruct args as [|a args'] eqn:E_args; destruct args0 as [|a0 args0'] eqn:E_args_0.
+        * simpl in H_cmp_sv1_sv2.
+          simpl.
+          destruct n.
+          ** exists (f ctx []). split; reflexivity.
+          ** simpl in H_follow_valid_sv1.
+             simpl in H_follow_valid_sv2.
+             destruct H_follow_valid_sv1 as [H_follow_valid_sv1_0 _].
+             unfold valid_stack_op_instr in H_follow_valid_sv1_0.
+             rewrite E_ops_label in H_follow_valid_sv1_0.
+             destruct H_follow_valid_sv1_0 as [H_follow_valid_sv1_0 _].
+             discriminate H_follow_valid_sv1_0.
+        * simpl in H_cmp_sv1_sv2. destruct H_comm; discriminate.
+        * simpl in H_cmp_sv1_sv2. destruct H_comm; try discriminate. destruct args'; try discriminate.
+          destruct args'; try discriminate.
+        * simpl in H_cmp_sv1_sv2. destruct H_comm; try discriminate.
+          destruct args' as [| a' args'']; try discriminate.                                                      
+          destruct args'' as [| a'' args''']; try discriminate.
+          destruct args0' as [| a0' args0'']; try discriminate.
+          destruct args0'' as [| a0'' args0''']; try discriminate.
+      + unfold safe_sha3_cmp_ext_d in H_safe_sha3_cmp.
+        pose proof (H_safe_sha3_cmp 0 (Nat.le_refl 0)) as H_safe_sha3_cmp.
+        simpl in H_safe_sha3_cmp.
+        unfold safe_sha3_cmp in H_safe_sha3_cmp.
+
+        simpl in H_follow_valid_sv1.
+        destruct H_follow_valid_sv1 as [ [H_follow_valid_offset [H_follow_valid_size H_follow_valid_smem]] [H_follow_valid_sb1' H_maxidx1_gt_maxidx1']].
+        pose proof (H_maxidx1_gt_maxidx1' (eq_refl true)) as  H_maxidx1_gt_maxidx1'.
+        
+        simpl in H_follow_valid_sv2.
+        destruct H_follow_valid_sv2 as [ [H_follow_valid_offset0 [H_follow_valid_size0 H_follow_valid_smem0]] [H_follow_valid_sb2' H_maxidx2_gt_maxidx2']].
+        pose proof (H_maxidx2_gt_maxidx2' (eq_refl true)) as  H_maxidx2_gt_maxidx2'.
+        
+        
+        pose proof (H_safe_sha3_cmp offset size smem offset0 size0 smem0 maxidx1' sb1' maxidx2' sb2' instk_height ops H_follow_valid_offset H_follow_valid_size H_follow_valid_offset0 H_follow_valid_size0 H_follow_valid_sb1' H_follow_valid_sb2' H_follow_valid_smem H_follow_valid_smem0 H_cmp_sv1_sv2 stk mem strg ctx H_len_stk) as H_safe_sha3_cmp.
+        
+        destruct H_safe_sha3_cmp as [coffset [csize [mem1 [coffset0 [csize0 [mem2 [v [H_eval_smem [H_eval_smem0 [H_eval_offset [H_eval_size [H_eval_offset0 [H_eval_size0 [H_sha3_mem1 H_sha3_mem2]]]]]]]]]]]]]].
+
+        unfold eval_smemory in H_eval_smem.
+        destruct (map_option (EvalCommon.instantiate_memory_update (fun sv : sstack_val => eval_sstack_val sv stk mem strg ctx maxidx1' sb1' ops)) smem) as [updates|] eqn:H_eval_smem_0; try discriminate.
+        unfold eval_sstack_val in H_eval_smem_0.
+        assert (H_maxidx1_ge_S_maxidx1': S maxidx1' <= maxidx1). intuition.
+        pose proof (instantiate_memory_update_mapo_preserved_when_depth_ext_le smem (S maxidx1') maxidx1 stk mem strg ctx maxidx1' sb1' ops updates H_maxidx1_ge_S_maxidx1' H_eval_smem_0) as H_eval_smem_0_ext.
+        rewrite H_eval_smem_0_ext.
+        
+        unfold eval_smemory in H_eval_smem0.
+        destruct (map_option (EvalCommon.instantiate_memory_update (fun sv : sstack_val => eval_sstack_val sv stk mem strg ctx maxidx2' sb2' ops)) smem0) as [updates0|] eqn:H_eval_smem0_0; try discriminate.
+        unfold eval_sstack_val in H_eval_smem0_0.
+        assert (H_maxidx2_ge_S_maxidx2': S maxidx2' <= maxidx2). intuition.
+        pose proof (instantiate_memory_update_mapo_preserved_when_depth_ext_le smem0 (S maxidx2') maxidx2 stk mem strg ctx maxidx2' sb2' ops updates0 H_maxidx2_ge_S_maxidx2' H_eval_smem0_0) as H_eval_smem0_0_ext.
+        rewrite H_eval_smem0_0_ext.
+
+        unfold eval_sstack_val in H_eval_offset.
+        pose proof (eval_sstack_val'_preserved_when_depth_extended_le (S maxidx1') maxidx1 maxidx1' sb1' offset coffset stk mem strg ctx ops H_maxidx1_ge_S_maxidx1' H_eval_offset) as H_eval_offset_0.
+        rewrite H_eval_offset_0.
+
+        unfold eval_sstack_val in H_eval_size.
+        pose proof (eval_sstack_val'_preserved_when_depth_extended_le (S maxidx1') maxidx1 maxidx1' sb1' size csize stk mem strg ctx ops H_maxidx1_ge_S_maxidx1' H_eval_size) as H_eval_size_0.
+        rewrite H_eval_size_0.
+
+        unfold eval_sstack_val in H_eval_offset0.
+        pose proof (eval_sstack_val'_preserved_when_depth_extended_le (S maxidx2') maxidx2 maxidx2' sb2' offset0 coffset0 stk mem strg ctx ops H_maxidx2_ge_S_maxidx2' H_eval_offset0) as H_eval_offset0_0.
+        rewrite H_eval_offset0_0.
+
+        unfold eval_sstack_val in H_eval_size0.
+        pose proof (eval_sstack_val'_preserved_when_depth_extended_le (S maxidx2') maxidx2 maxidx2' sb2' size0 csize0 stk mem strg ctx ops H_maxidx2_ge_S_maxidx2' H_eval_size0) as H_eval_size0_0.
+        rewrite H_eval_size0_0.
+
+        injection H_eval_smem as H_eval_smem.
+        rewrite H_eval_smem.
+        injection H_eval_smem0 as H_eval_smem0.
+        rewrite H_eval_smem0.
+        
+        rewrite H_sha3_mem1.
+        rewrite H_sha3_mem2.
+        exists v.
+        split; reflexivity.
+
+    - intros smemory_cmp sstorage_cmp sha3_cmp H_safe_smemory_cmp H_safe_sstorage_cmp H_safe_sha3_cmp.
+      unfold safe_sstack_val_cmp_ext_2_d.
+      unfold safe_sstack_val_cmp_ext_1_d.
+      unfold safe_sstack_val_cmp.
+      intros d'0 H_d'0_le_SS_d'.
+      intros sv1 sv2 maxidx1 sb1 maxidx2 sb2 instk_height ops H_valid_sv1 H_valid_sv2 H_valid_sb1 H_valid_sb2 H_cmp_sv1_sv2.
+      intros stk mem strg ctx H_len_stk.
+      destruct d'0; try discriminate.
+      simpl in H_cmp_sv1_sv2.
+      unfold eval_sstack_val.
+      
+      destruct (match sv1 with
+                    | Val w1 => match sv2 with
+                                | Val w2 => weqb w1 w2
+                                | _ => false
+                                end
+                    | InStackVar n1 =>
+                        match sv2 with
+                        | InStackVar n2 => (n1 =? n2) && ((n1 <? instk_height) && (n2 <? instk_height))
+                        | _ => false
+                        end
+                    | FreshVar n1 =>
+                        match sv2 with
+                        | FreshVar n2 =>
+                            if n1 =? n2
+                            then
+                             if maxidx1 =? maxidx2
+                             then if sbindings_eq_dec sb1 sb2 then true else false
+                             else false
+                            else false
+                        | _ => false
+                        end
+                    end) eqn:E_trivial_chk.
+
+      (* when calling trivial check *)
+      destruct sv1 as [w1 | n1 | n1]; destruct sv2 as [w2 | n2 | n2] eqn:E_sv2; try discriminate.
+
+
+        (* Val *)
+        apply weqb_sound in E_trivial_chk.
+
+        pose proof (eval_sstack_val'_Val w1 stk mem strg ctx maxidx1 sb1 ops) as H_eval_w1.
+        pose proof (eval_sstack_val'_Val w2 stk mem strg ctx maxidx2 sb2 ops) as H_eval_w2.
+        rewrite H_eval_w1.
+        rewrite H_eval_w2.
+        rewrite E_trivial_chk.
+        exists w2.
+        split; reflexivity.
+
+
+        (* InStackVar *)
+        pose proof (eval_sstack_val'_InStackVar n1 stk mem strg ctx maxidx1 sb1 ops) as H_eval_instkv_n1.
+        pose proof (eval_sstack_val'_InStackVar n2 stk mem strg ctx maxidx2 sb2 ops) as H_eval_instkv_n2.
+        rewrite H_eval_instkv_n1.
+        rewrite H_eval_instkv_n2.
+
+        apply andb_prop in E_trivial_chk.
+        destruct E_trivial_chk as [E_trivial_chk_1 E_trivial_chk].
+        apply andb_prop in E_trivial_chk.
+        destruct E_trivial_chk as [E_trivial_chk_2 E_trivial_chk_3].
+        
+        apply Nat.eqb_eq in E_trivial_chk_1.
+        apply Nat.ltb_lt in E_trivial_chk_2.
+        apply Nat.ltb_lt in E_trivial_chk_3.
+
+        rewrite <- H_len_stk in E_trivial_chk_3.
+        
+        pose proof (nth_error_ok' EVMWord stk n2 E_trivial_chk_3) as H_nth_error_ok'.
+        destruct  H_nth_error_ok' as [v'  H_nth_error_ok'].
+        
+        rewrite E_trivial_chk_1.
+        rewrite H_nth_error_ok'.
+        exists v'.
+        split; try reflexivity.
+        
+        (* FreshVar *)
+        destruct (n1 =? n2) eqn:E_n1_eq_n2; try discriminate.
+        destruct (maxidx1 =? maxidx2) eqn:E_maxidx1_eq_maxidx2; try discriminate.
+        destruct (sbindings_eq_dec sb1 sb2) eqn:E_bs1_eq_bs2; try discriminate.
+        apply Nat.eqb_eq in E_n1_eq_n2.
+        apply Nat.eqb_eq in E_maxidx1_eq_maxidx2.
+
+        rewrite E_n1_eq_n2.
+        rewrite E_maxidx1_eq_maxidx2.
+        rewrite e.
+                  
+        pose proof (eval_sstack_val'_succ (S maxidx2) instk_height (FreshVar n2) stk mem strg ctx maxidx2 sb2 ops (eq_sym H_len_stk) H_valid_sv2 H_valid_sb2 (gt_Sn_n maxidx2)) as H_eval_sv2.
+        destruct H_eval_sv2 as [v2 H_eval_sv2].
+
+        rewrite H_eval_sv2.
+        exists v2.
+        split; try reflexivity.
+      (* end of call to trivial chk *)
+
+ 
+      
+      unfold eval_sstack_val'. fold eval_sstack_val'.
+
+      assert(H_d'_le_Sd': d' <= S d'). intuition.
+
+      pose proof (safe_smemory_cmp_ext_d_lt smemory_cmp (basic_compare_sstack_val_w_eq_chk smemory_cmp sstorage_cmp sha3_cmp) d'  (S d') H_d'_le_Sd' H_safe_smemory_cmp) as H_safe_smemory_cmp_d'.
+      pose proof (safe_sstorage_cmp_ext_d_lt sstorage_cmp (basic_compare_sstack_val_w_eq_chk smemory_cmp sstorage_cmp sha3_cmp) d'  (S d') H_d'_le_Sd' H_safe_sstorage_cmp) as H_safe_sstorgae_cmp_d'.
+      pose proof (safe_sha3_cmp_ext_d_lt sha3_cmp (basic_compare_sstack_val_w_eq_chk smemory_cmp sstorage_cmp sha3_cmp) d'  (S d') H_d'_le_Sd' H_safe_sha3_cmp) as H_safe_sha3_cmp_d'.
+      pose proof (IHd' smemory_cmp sstorage_cmp sha3_cmp H_safe_smemory_cmp_d' H_safe_sstorgae_cmp_d' H_safe_sha3_cmp_d') as H_safe_sstack_value_cmp_cmp_Sd'.
+      
+      assert(H_d'0_le_Sd': d'0 <= S d'). intuition.
+        
+
+      pose proof (safe_sstack_val_cmp_ext_2_d_le basic_compare_sstack_val_w_eq_chk smemory_cmp sstorage_cmp sha3_cmp d'0 (S d') H_d'0_le_Sd' H_safe_sstack_value_cmp_cmp_Sd') as H_safe_sstack_value_cmp_cmp_d'0.
+
+      pose proof (follow_in_smap_suc sb1 sv1 instk_height maxidx1 ops H_valid_sv1 H_valid_sb1) as H_follow_suc_sv1.
+      destruct H_follow_suc_sv1 as [smv1 [maxidx1' [sb1' [H_follow_suc_sv1 _]]]].
+      pose proof (follow_in_smap_suc sb2 sv2 instk_height maxidx2 ops H_valid_sv2 H_valid_sb2) as H_follow_suc_sv2.
+      destruct H_follow_suc_sv2 as [smv2 [maxidx2' [sb2' [H_follow_suc_sv2 _]]]].
+
+      rewrite H_follow_suc_sv1.
+      rewrite H_follow_suc_sv2.
+
+      rewrite H_follow_suc_sv1 in H_cmp_sv1_sv2.
+      rewrite H_follow_suc_sv2 in H_cmp_sv1_sv2.
+
+      pose proof (valid_follow_in_smap sb1 sv1 instk_height maxidx1 ops smv1 maxidx1' sb1' H_valid_sv1 H_valid_sb1 H_follow_suc_sv1) as H_follow_valid_sv1.
+      pose proof (valid_follow_in_smap sb2 sv2 instk_height maxidx2 ops smv2 maxidx2' sb2' H_valid_sv2 H_valid_sb2 H_follow_suc_sv2) as H_follow_valid_sv2.
+ 
+      destruct smv1 eqn:E_smv1; destruct smv2 eqn:E_smv2; try discriminate.
+      
+      + destruct val; destruct val0; try discriminate.
+        * apply weqb_sound in H_cmp_sv1_sv2.
+          rewrite H_cmp_sv1_sv2.
+          exists val0.
+          split; reflexivity.
+        * apply andb_prop in H_cmp_sv1_sv2 as [H_var_va0 H_cmp_sv1_sv2].
+          apply andb_prop in H_cmp_sv1_sv2 as [H_var_lt_inskt H_var0_lt_instk].
+          apply Nat.eqb_eq in H_var_va0.
+          rewrite H_var_va0.
+          rewrite <- H_len_stk in H_var0_lt_instk.
+          apply Nat.ltb_lt in H_var0_lt_instk.
+          pose proof (nth_error_nth' stk WZero H_var0_lt_instk) as H_nth_error.
+          rewrite H_nth_error.
+          exists (nth var0 stk WZero).
+          split; reflexivity.
+      + apply andb_prop in H_cmp_sv1_sv2 as [H_cmp_sv1_sv2_0 H_cmp_sv1_sv2_1].
+        apply N.eqb_eq in H_cmp_sv1_sv2_0.
+        apply N.eqb_eq in H_cmp_sv1_sv2_1.
+        rewrite H_cmp_sv1_sv2_0.
+        rewrite H_cmp_sv1_sv2_1.
+        exists (get_tags_ctx ctx cat0 val0). split; reflexivity.
+      + fold eval_sstack_val' in H_cmp_sv1_sv2. destruct (label =?i label0) eqn:E_eqb_label_label0; try discriminate.
+        apply eqb_stack_op_instr_eq in E_eqb_label_label0 as E_eq_label_label0.
+        rewrite <- E_eq_label_label0.
+        rewrite <- E_eq_label_label0 in H_follow_suc_sv2.
+        rewrite <- E_eq_label_label0 in H_follow_valid_sv2.
+
+        destruct H_follow_valid_sv1 as [H_follow_valid_sv1_0 [H_follow_valid_sv1_1 H_follow_valid_sv1_2]].
+        simpl in H_follow_valid_sv1_0.
+        unfold valid_stack_op_instr in H_follow_valid_sv1_0.
+        destruct (ops label) eqn:E_ops_label.
+        destruct H_follow_valid_sv1_0 as [H_follow_valid_sv1_0_0 H_follow_valid_sv1_0_1].
+
+        destruct H_follow_valid_sv2 as [H_follow_valid_sv2_0 [H_follow_valid_sv2_1 H_follow_valid_sv2_2]].
+        simpl in H_follow_valid_sv2_0.
+        unfold valid_stack_op_instr in H_follow_valid_sv2_0.
+        rewrite E_ops_label in H_follow_valid_sv2_0.
+        destruct H_follow_valid_sv2_0 as [H_follow_valid_sv2_0_0 H_follow_valid_sv2_0_1].
+
+        apply Nat.eqb_eq in H_follow_valid_sv1_0_0 as H_follow_valid_sv1_0_0_eq.
+        apply Nat.eqb_eq in H_follow_valid_sv2_0_0 as H_follow_valid_sv2_0_0_eq.
+
+        rewrite H_follow_valid_sv1_0_0_eq.
+        rewrite H_follow_valid_sv2_0_0_eq.
+        assert(H_follow_valid_sv1_0_0_eq' := H_follow_valid_sv1_0_0_eq).
+        rewrite <- H_follow_valid_sv2_0_0 in H_follow_valid_sv1_0_0_eq'.
+        
+        unfold safe_sstack_val_cmp_ext_2_d in H_safe_sstack_value_cmp_cmp_d'0.
+        unfold safe_sstack_val_cmp_ext_1_d in H_safe_sstack_value_cmp_cmp_d'0.
+        unfold safe_sstack_val_cmp in H_safe_sstack_value_cmp_cmp_d'0.
+        
+        assert(H_fldr:
+                forall args1 args2,
+                  valid_sstack instk_height maxidx1' args1 ->
+                  valid_sstack instk_height maxidx2' args2 ->
+                  fold_right_two_lists (fun e1 e2 : sstack_val => basic_compare_sstack_val_w_eq_chk smemory_cmp sstorage_cmp sha3_cmp d'0 e1 e2 maxidx1' sb1' maxidx2' sb2' instk_height ops) args1 args2 = true ->
+                  exists args',
+                    map_option (fun sv' : sstack_val => eval_sstack_val' (S maxidx1') sv' stk mem strg ctx maxidx1' sb1' ops) args1 = Some args' /\
+                      map_option (fun sv' : sstack_val => eval_sstack_val' (S maxidx2') sv' stk mem strg ctx maxidx2' sb2' ops) args2 = Some args').
+        (* staring proof of assert *)
+        * induction args1 as [|a1_1 args1'].
+          ** destruct args2 as [|a1_2 args2']; try discriminate.
+             intros.
+             simpl.
+             exists [].
+             split; reflexivity.
+          ** destruct args2 as [|a1_2 args2']; try discriminate.
+             intros H_valid_sstack_args1 H_valid_sstack_args2 H_fldr.
+             unfold fold_right_two_lists in H_fldr.
+             rewrite <- fold_right_two_lists_ho in H_fldr.
+             destruct (basic_compare_sstack_val_w_eq_chk smemory_cmp sstorage_cmp sha3_cmp d'0 a1_1 a1_2
+                         maxidx1' sb1' maxidx2' sb2' instk_height ops) eqn:E_cmp_a1_1_a1_2; try discriminate.
+             simpl in H_valid_sstack_args1.
+             destruct H_valid_sstack_args1 as [H_valid_a1_1 H_valid_arg1'].
+             simpl in H_valid_sstack_args2.
+             destruct H_valid_sstack_args2 as [H_valid_a1_2 H_valid_arg2'].
+             
+             pose proof (H_safe_sstack_value_cmp_cmp_d'0 d'0 (Nat.le_refl d'0) a1_1 a1_2 maxidx1' sb1' maxidx2' sb2' instk_height ops H_valid_a1_1 H_valid_a1_2 H_follow_valid_sv1_1 H_follow_valid_sv2_1 E_cmp_a1_1_a1_2 stk mem strg ctx H_len_stk) as H_eval_sstack_value_a1_1_a1_2.
+             destruct H_eval_sstack_value_a1_1_a1_2 as [v [H_eval_sstack_value_a1_1 H_eval_sstack_value_a1_2]].
+
+             unfold eval_sstack_val in H_eval_sstack_value_a1_1.
+             unfold eval_sstack_val in H_eval_sstack_value_a1_2.
+             unfold map_option.
+             repeat rewrite <- map_option_ho.
+             rewrite H_eval_sstack_value_a1_1.
+             rewrite H_eval_sstack_value_a1_2.
+             pose proof (IHargs1' args2' H_valid_arg1'  H_valid_arg2' H_fldr) as H_mapo.
+             destruct H_mapo as [args' [H_mapo_args1' H_mapo_args2']].
+             rewrite H_mapo_args1'.
+             rewrite H_mapo_args2'.
+             exists (v :: args').
+             split; reflexivity.
+        (* ending proof of assert *)
+        * destruct (fold_right_two_lists
+                      (fun e1 e2 : sstack_val =>
+                       basic_compare_sstack_val_w_eq_chk smemory_cmp sstorage_cmp sha3_cmp d'0 e1 e2 maxidx1' sb1' maxidx2' sb2'
+                         instk_height ops) args args0) eqn:E_fldr.
+          ** pose proof (H_fldr args args0 H_follow_valid_sv1_0_1 H_follow_valid_sv2_0_1 E_fldr) as H_fldr_0.
+             destruct H_fldr_0 as [args' [H_fldr_0_0 H_fldr_0_1]].
+             
+             simpl in H_follow_valid_sv2_2.
+             pose proof (H_follow_valid_sv2_2 (eq_refl true)) as H_follow_valid_sv2_2.
+             
+             simpl in H_follow_valid_sv1_2.
+             pose proof (H_follow_valid_sv1_2 (eq_refl true)) as H_follow_valid_sv1_2.
+             assert (H_maxidx1_ge_S_maxidx1': maxidx1 >= S maxidx1'). intuition.
+             
+             pose proof (eval_sstack_val'_mapo_preserved_when_depth_ext_le args (S maxidx1') maxidx1 stk mem strg ctx maxidx1' sb1' ops args' H_maxidx1_ge_S_maxidx1' H_fldr_0_0) as H_fldr_0_0_0.
+             rewrite H_fldr_0_0_0.
+
+             assert (H_maxidx2_ge_S_maxidx2': maxidx2 >= S maxidx2'). intuition.
+             pose proof (eval_sstack_val'_mapo_preserved_when_depth_ext_le args0 (S maxidx2') maxidx2 stk mem strg ctx maxidx2' sb2' ops args' H_maxidx2_ge_S_maxidx2' H_fldr_0_1) as H_fldr_0_1_0.
+             rewrite H_fldr_0_1_0.
+             exists (f ctx args').
+             split; reflexivity.
+          ** destruct H_comm as [H_f_comm_proof|]; try discriminate.
+
+             destruct args as [|a1 args]; try discriminate.
+             destruct args as [|a2 args]; try discriminate.
+             destruct args; try discriminate.
+             destruct args0 as [|b1 args0]; try discriminate.
+             destruct args0 as [|b2 args0]; try discriminate.
+             destruct args0; try discriminate.
+
+             destruct (basic_compare_sstack_val_w_eq_chk smemory_cmp sstorage_cmp sha3_cmp d'0 a1 b2 maxidx1' sb1' maxidx2' sb2' instk_height ops) eqn:E_cmp_a1_b2; try discriminate.
+
+             simpl in H_follow_valid_sv1_0_1.
+             destruct H_follow_valid_sv1_0_1 as [H_follow_valid_a1 [H_follow_valid_a2 _]].
+             simpl in H_follow_valid_sv2_0_1.
+             destruct H_follow_valid_sv2_0_1 as [H_follow_valid_b1 [H_follow_valid_b2 _]].
+             
+             pose proof (H_safe_sstack_value_cmp_cmp_d'0 d'0 (Nat.le_refl d'0) a1 b2 maxidx1' sb1' maxidx2' sb2' instk_height ops H_follow_valid_a1 H_follow_valid_b2 H_follow_valid_sv1_1 H_follow_valid_sv2_1 E_cmp_a1_b2 stk mem strg ctx H_len_stk) as H_safe_sstack_value_cmp_a1_b2.
+             unfold eval_sstack_val in H_safe_sstack_value_cmp_a1_b2.
+             destruct H_safe_sstack_value_cmp_a1_b2 as [v1 [H_safe_sstack_value_cmp_a1 H_safe_sstack_value_cmp_b2]].
+
+             pose proof (H_safe_sstack_value_cmp_cmp_d'0 d'0 (Nat.le_refl d'0) a2 b1 maxidx1' sb1' maxidx2' sb2' instk_height ops H_follow_valid_a2 H_follow_valid_b1 H_follow_valid_sv1_1 H_follow_valid_sv2_1 H_cmp_sv1_sv2 stk mem strg ctx H_len_stk) as H_safe_sstack_value_cmp_a2_b1.
+             unfold eval_sstack_val in H_safe_sstack_value_cmp_a2_b1.
+             destruct H_safe_sstack_value_cmp_a2_b1 as [v2 [H_safe_sstack_value_cmp_a2 H_safe_sstack_value_cmp_b1]].
+
+             assert(H_Smaxidx1'_le_maxidx1: S maxidx1' <= maxidx1). intuition.
+             pose proof (eval_sstack_val'_preserved_when_depth_extended_le (S maxidx1') maxidx1 maxidx1' sb1' a1 v1 stk mem strg ctx ops H_Smaxidx1'_le_maxidx1 H_safe_sstack_value_cmp_a1) as H_safe_sstack_value_cmp_a1_ext.
+
+             assert(H_Smaxidx2'_le_maxidx2: S maxidx2' <= maxidx2). intuition.
+             pose proof (eval_sstack_val'_preserved_when_depth_extended_le (S maxidx2') maxidx2 maxidx2' sb2' b2 v1 stk mem strg ctx ops H_Smaxidx2'_le_maxidx2 H_safe_sstack_value_cmp_b2) as H_safe_sstack_value_cmp_b2_ext.
+
+
+             pose proof (eval_sstack_val'_preserved_when_depth_extended_le (S maxidx1') maxidx1 maxidx1' sb1' a2 v2 stk mem strg ctx ops H_Smaxidx1'_le_maxidx1 H_safe_sstack_value_cmp_a2) as H_safe_sstack_value_cmp_a2_ext.
+
+             pose proof (eval_sstack_val'_preserved_when_depth_extended_le (S maxidx2') maxidx2 maxidx2' sb2' b1 v2 stk mem strg ctx ops H_Smaxidx2'_le_maxidx2 H_safe_sstack_value_cmp_b1) as H_safe_sstack_value_cmp_b1_ext.
+
+             unfold map_option.
+             rewrite H_safe_sstack_value_cmp_a1_ext.
+             rewrite H_safe_sstack_value_cmp_b2_ext.
+             rewrite H_safe_sstack_value_cmp_a2_ext.
+             rewrite H_safe_sstack_value_cmp_b1_ext.
+
+             exists (f ctx [v1; v2]).
+
+             unfold commutative_op in H_f_comm_proof.
+             rewrite H_f_comm_proof.
+             split; reflexivity.
+      + destruct (basic_compare_sstack_val_w_eq_chk smemory_cmp sstorage_cmp sha3_cmp d'0 offset offset0 maxidx1' sb1' maxidx2' sb2' instk_height ops) eqn:E_cmp_offset_offset0; try discriminate.
+
+        simpl in H_follow_valid_sv1.
+        destruct H_follow_valid_sv1 as [[H_valid_offset H_valid_smem] [H_valid_sb1' H_maxidx1_gt_maxidx1']].
+        pose proof (H_maxidx1_gt_maxidx1' (eq_refl true)) as H_maxidx1_gt_maxidx1'.
+
+        simpl in H_follow_valid_sv2.
+        destruct H_follow_valid_sv2 as [[H_valid_offset0 H_valid_smem0] [H_valid_sb2' H_maxidx2_gt_maxidx2']].
+        pose proof (H_maxidx2_gt_maxidx2' (eq_refl true)) as H_maxidx2_gt_maxidx2'.
+
+
+        pose proof (H_safe_sstack_value_cmp_cmp_d'0 d'0 (Nat.le_refl d'0) offset offset0 maxidx1' sb1' maxidx2' sb2' instk_height ops H_valid_offset H_valid_offset0 H_valid_sb1' H_valid_sb2' E_cmp_offset_offset0 stk mem strg ctx H_len_stk) as H_eval_offset_offset0.
+        unfold eval_sstack_val in H_eval_offset_offset0.
+        destruct H_eval_offset_offset0 as [v [H_eval_offset H_eval_offset0]].
+        
+
+        assert (H_Smaxidx1'_le_maxidx1: S maxidx1' <= maxidx1). intuition.
+        pose proof (eval_sstack_val'_preserved_when_depth_extended_le (S maxidx1') maxidx1 maxidx1' sb1' offset v stk mem strg ctx ops H_Smaxidx1'_le_maxidx1 H_eval_offset) as H_eval_soffset_ext.
+        rewrite H_eval_soffset_ext.
+        assert (H_Smaxidx2'_le_maxidx2: S maxidx2' <= maxidx2). intuition.
+        pose proof (eval_sstack_val'_preserved_when_depth_extended_le (S maxidx2') maxidx2 maxidx2' sb2' offset0 v stk mem strg ctx ops H_Smaxidx2'_le_maxidx2 H_eval_offset0) as H_eval_soffset0_ext.
+        rewrite H_eval_soffset0_ext.
+
+        unfold safe_smemory_cmp_ext_d in H_safe_smemory_cmp.
+        unfold safe_smemory_cmp in H_safe_smemory_cmp.
+
+        assert(H_d'0_le_d': d'0 <= S d'). intuition.
+
+        pose proof (H_safe_smemory_cmp d'0 H_d'0_le_d' smem smem0 maxidx1' sb1' maxidx2' sb2' instk_height ops H_valid_sb1' H_valid_sb2' H_valid_smem H_valid_smem0 H_cmp_sv1_sv2 stk mem strg ctx H_len_stk) as H_safe_smemory_cmp_0.
+
+        destruct H_safe_smemory_cmp_0 as [mem' [H_eval_mem H_eval_mem0]].
+        unfold eval_smemory in H_eval_mem.
+        unfold eval_smemory in H_eval_mem0.
+
+
+        destruct (map_option
+                   (instantiate_memory_update
+                      (fun sv : sstack_val =>
+                       eval_sstack_val sv stk mem strg ctx maxidx1'
+                         sb1' ops)) smem) as [updates|] eqn:E_mapo_mem; try discriminate.
+        unfold eval_sstack_val in E_mapo_mem.
+        
+        destruct (map_option
+                    (instantiate_memory_update
+                       (fun sv : sstack_val =>
+                        eval_sstack_val sv stk mem strg ctx maxidx2'
+                          sb2' ops)) smem0) as [updates0|] eqn:E_mapo_mem0; try discriminate.
+        unfold eval_sstack_val in E_mapo_mem0.
+
+        pose proof (instantiate_memory_update_mapo_preserved_when_depth_ext_le smem (S maxidx1') maxidx1 stk mem strg ctx maxidx1' sb1' ops updates H_Smaxidx1'_le_maxidx1 E_mapo_mem) as E_mapo_mem_ext.
+        rewrite E_mapo_mem_ext.
+        
+        pose proof (instantiate_memory_update_mapo_preserved_when_depth_ext_le smem0 (S maxidx2') maxidx2 stk mem strg ctx maxidx2' sb2' ops updates0 H_Smaxidx2'_le_maxidx2 E_mapo_mem0) as E_mapo_mem0_ext.
+        rewrite E_mapo_mem0_ext.
+
+        injection H_eval_mem0 as H_eval_mem0.
+        injection H_eval_mem as H_eval_mem.
+
+        rewrite H_eval_mem0.
+        rewrite H_eval_mem.
+
+        exists (concrete_interpreter.ConcreteInterpreter.mload mem' v).
+        split; reflexivity.
+        
+      + destruct (basic_compare_sstack_val_w_eq_chk smemory_cmp sstorage_cmp sha3_cmp d'0 key key0 maxidx1' sb1' maxidx2' sb2' instk_height ops) eqn:E_cmp_key_key0; try discriminate.
+
+        simpl in H_follow_valid_sv1.
+        destruct H_follow_valid_sv1 as [[H_valid_key H_valid_sstrg] [H_valid_sb1' H_maxidx1_gt_maxidx1']].
+        pose proof (H_maxidx1_gt_maxidx1' (eq_refl true)) as H_maxidx1_gt_maxidx1'.
+
+        simpl in H_follow_valid_sv2.
+        destruct H_follow_valid_sv2 as [[H_valid_key0 H_valid_sstrg0] [H_valid_sb2' H_maxidx2_gt_maxidx2']].
+        pose proof (H_maxidx2_gt_maxidx2' (eq_refl true)) as H_maxidx2_gt_maxidx2'.
+
+
+        pose proof (H_safe_sstack_value_cmp_cmp_d'0 d'0 (Nat.le_refl d'0) key key0 maxidx1' sb1' maxidx2' sb2' instk_height ops H_valid_key H_valid_key0 H_valid_sb1' H_valid_sb2' E_cmp_key_key0 stk mem strg ctx H_len_stk) as H_eval_key_key0.
+        unfold eval_sstack_val in H_eval_key_key0.
+        destruct H_eval_key_key0 as [v [H_eval_key H_eval_key0]].
+        
+
+        assert (H_Smaxidx1'_le_maxidx1: S maxidx1' <= maxidx1). intuition.
+        pose proof (eval_sstack_val'_preserved_when_depth_extended_le (S maxidx1') maxidx1 maxidx1' sb1' key v stk mem strg ctx ops H_Smaxidx1'_le_maxidx1 H_eval_key) as H_eval_skey_ext.
+        rewrite H_eval_skey_ext.
+        assert (H_Smaxidx2'_le_maxidx2: S maxidx2' <= maxidx2). intuition.
+        pose proof (eval_sstack_val'_preserved_when_depth_extended_le (S maxidx2') maxidx2 maxidx2' sb2' key0 v stk mem strg ctx ops H_Smaxidx2'_le_maxidx2 H_eval_key0) as H_eval_skey0_ext.
+        rewrite H_eval_skey0_ext.
+
+        unfold safe_sstorage_cmp_ext_d in H_safe_sstorage_cmp.
+        unfold safe_sstorage_cmp in H_safe_sstorage_cmp.
+
+        assert(H_d'0_le_d': d'0 <= S d'). intuition.
+
+        pose proof (H_safe_sstorage_cmp d'0 H_d'0_le_d' sstrg sstrg0 maxidx1' sb1' maxidx2' sb2' instk_height ops H_valid_sb1' H_valid_sb2' H_valid_sstrg H_valid_sstrg0 H_cmp_sv1_sv2 stk mem strg ctx H_len_stk) as H_safe_sstorage_cmp_0.
+
+        destruct H_safe_sstorage_cmp_0 as [strg' [H_eval_sstrg H_eval_sstrg0]].
+        unfold eval_sstorage in H_eval_sstrg.
+        unfold eval_sstorage in H_eval_sstrg0.
+
+
+        destruct (map_option
+                   (instantiate_storage_update
+                      (fun sv : sstack_val =>
+                       eval_sstack_val sv stk mem strg ctx maxidx1'
+                         sb1' ops)) sstrg) as [updates|] eqn:E_mapo_strg; try discriminate.
+        unfold eval_sstack_val in E_mapo_strg.
+        
+        destruct (map_option
+                    (instantiate_storage_update
+                       (fun sv : sstack_val =>
+                        eval_sstack_val sv stk mem strg ctx maxidx2'
+                          sb2' ops)) sstrg0) as [updates0|] eqn:E_mapo_strg0; try discriminate.
+        unfold eval_sstack_val in E_mapo_strg0.
+
+        pose proof (instantiate_storage_update_mapo_preserved_when_depth_ext_le sstrg (S maxidx1') maxidx1 stk mem strg ctx maxidx1' sb1' ops updates H_Smaxidx1'_le_maxidx1 E_mapo_strg) as E_mapo_strg_ext.
+        rewrite E_mapo_strg_ext.
+        
+        pose proof (instantiate_storage_update_mapo_preserved_when_depth_ext_le sstrg0 (S maxidx2') maxidx2 stk mem strg ctx maxidx2' sb2' ops updates0 H_Smaxidx2'_le_maxidx2 E_mapo_strg0) as E_mapo_strg0_ext.
+        rewrite E_mapo_strg0_ext.
+
+        injection H_eval_sstrg0 as H_eval_sstrg0.
+        injection H_eval_sstrg as H_eval_sstrg.
+
+        rewrite H_eval_sstrg0.
+        rewrite H_eval_sstrg.
+
+        exists (concrete_interpreter.ConcreteInterpreter.sload strg' v).
+        split; reflexivity.
+
+      + assert(H_d'0_le_d': d'0 <= S d'). intuition.
+        assert (H_Smaxidx1'_le_maxidx1: S maxidx1' <= maxidx1). intuition.
+        assert (H_Smaxidx2'_le_maxidx2: S maxidx2' <= maxidx2). intuition.
+
+        simpl in H_follow_valid_sv1.
+        destruct H_follow_valid_sv1 as [[H_valid_offset [H_valid_size H_valid_smem]] [H_valid_sb1' H_maxidx1_gt_maxidx1']].
+        pose proof (H_maxidx1_gt_maxidx1' (eq_refl true)) as H_maxidx1_gt_maxidx1'.
+
+        simpl in H_follow_valid_sv2.
+        destruct H_follow_valid_sv2 as [[H_valid_offset0 [H_valid_size0 H_valid_smem0]] [H_valid_sb2' H_maxidx2_gt_maxidx2']].
+        pose proof (H_maxidx2_gt_maxidx2' (eq_refl true)) as H_maxidx2_gt_maxidx2'.
+
+        destruct (if
+                     basic_compare_sstack_val_w_eq_chk smemory_cmp sstorage_cmp sha3_cmp d'0 offset offset0 maxidx1' sb1'
+                       maxidx2' sb2' instk_height ops
+                    then
+                     if
+                      basic_compare_sstack_val_w_eq_chk smemory_cmp sstorage_cmp sha3_cmp d'0 size size0 maxidx1' sb1'
+                        maxidx2' sb2' instk_height ops
+                     then
+                       smemory_cmp (basic_compare_sstack_val_w_eq_chk smemory_cmp sstorage_cmp sha3_cmp d'0) smem smem0
+                         maxidx1' sb1' maxidx2' sb2' instk_height ops
+                     else false
+                   else false) eqn:E_std_sha3.
+
+        * destruct (basic_compare_sstack_val_w_eq_chk smemory_cmp sstorage_cmp sha3_cmp d'0 offset offset0 maxidx1' sb1' maxidx2' sb2' instk_height ops) eqn:E_cmp_offset_offset0; try discriminate.
+          destruct (basic_compare_sstack_val_w_eq_chk smemory_cmp sstorage_cmp sha3_cmp d'0 size size0 maxidx1' sb1' maxidx2' sb2' instk_height ops) eqn:E_cmp_size_size0; try discriminate.
+
+
+
+        pose proof (H_safe_sstack_value_cmp_cmp_d'0 d'0 (Nat.le_refl d'0) offset offset0 maxidx1' sb1' maxidx2' sb2' instk_height ops H_valid_offset H_valid_offset0 H_valid_sb1' H_valid_sb2' E_cmp_offset_offset0 stk mem strg ctx H_len_stk) as H_eval_offset_offset0.
+        unfold eval_sstack_val in H_eval_offset_offset0.
+        destruct H_eval_offset_offset0 as [v [H_eval_offset H_eval_offset0]].
+        
+
+        pose proof (eval_sstack_val'_preserved_when_depth_extended_le (S maxidx1') maxidx1 maxidx1' sb1' offset v stk mem strg ctx ops H_Smaxidx1'_le_maxidx1 H_eval_offset) as H_eval_soffset_ext.
+        rewrite H_eval_soffset_ext.
+        pose proof (eval_sstack_val'_preserved_when_depth_extended_le (S maxidx2') maxidx2 maxidx2' sb2' offset0 v stk mem strg ctx ops H_Smaxidx2'_le_maxidx2 H_eval_offset0) as H_eval_soffset0_ext.
+        rewrite H_eval_soffset0_ext.
+
+
+        pose proof (H_safe_sstack_value_cmp_cmp_d'0 d'0 (Nat.le_refl d'0) size size0 maxidx1' sb1' maxidx2' sb2' instk_height ops H_valid_size H_valid_size0 H_valid_sb1' H_valid_sb2' E_cmp_size_size0 stk mem strg ctx H_len_stk) as H_eval_size_size0.
+        unfold eval_sstack_val in H_eval_size_size0.
+        destruct H_eval_size_size0 as [v' [H_eval_size H_eval_size0]].
+        
+
+        pose proof (eval_sstack_val'_preserved_when_depth_extended_le (S maxidx1') maxidx1 maxidx1' sb1' size v' stk mem strg ctx ops H_Smaxidx1'_le_maxidx1 H_eval_size) as H_eval_ssize_ext.
+        rewrite H_eval_ssize_ext.
+        pose proof (eval_sstack_val'_preserved_when_depth_extended_le (S maxidx2') maxidx2 maxidx2' sb2' size0 v' stk mem strg ctx ops H_Smaxidx2'_le_maxidx2 H_eval_size0) as H_eval_ssize0_ext.
+        rewrite H_eval_ssize0_ext.
+
+        
+        unfold safe_smemory_cmp_ext_d in H_safe_smemory_cmp.
+        unfold safe_smemory_cmp in H_safe_smemory_cmp.
+
+
+        pose proof (H_safe_smemory_cmp d'0 H_d'0_le_d' smem smem0 maxidx1' sb1' maxidx2' sb2' instk_height ops H_valid_sb1' H_valid_sb2' H_valid_smem H_valid_smem0 E_std_sha3 stk mem strg ctx H_len_stk) as H_safe_smemory_cmp_0.
+
+        destruct H_safe_smemory_cmp_0 as [mem' [H_eval_mem H_eval_mem0]].
+        unfold eval_smemory in H_eval_mem.
+        unfold eval_smemory in H_eval_mem0.
+
+
+        destruct (map_option
+                   (instantiate_memory_update
+                      (fun sv : sstack_val =>
+                       eval_sstack_val sv stk mem strg ctx maxidx1'
+                         sb1' ops)) smem) as [updates|] eqn:E_mapo_mem; try discriminate.
+        unfold eval_sstack_val in E_mapo_mem.
+        
+        destruct (map_option
+                    (instantiate_memory_update
+                       (fun sv : sstack_val =>
+                        eval_sstack_val sv stk mem strg ctx maxidx2'
+                          sb2' ops)) smem0) as [updates0|] eqn:E_mapo_mem0; try discriminate.
+        unfold eval_sstack_val in E_mapo_mem0.
+
+        pose proof (instantiate_memory_update_mapo_preserved_when_depth_ext_le smem (S maxidx1') maxidx1 stk mem strg ctx maxidx1' sb1' ops updates H_Smaxidx1'_le_maxidx1 E_mapo_mem) as E_mapo_mem_ext.
+        rewrite E_mapo_mem_ext.
+        
+        pose proof (instantiate_memory_update_mapo_preserved_when_depth_ext_le smem0 (S maxidx2') maxidx2 stk mem strg ctx maxidx2' sb2' ops updates0 H_Smaxidx2'_le_maxidx2 E_mapo_mem0) as E_mapo_mem0_ext.
+        rewrite E_mapo_mem0_ext.
+
+        injection H_eval_mem0 as H_eval_mem0.
+        injection H_eval_mem as H_eval_mem.
+
+        rewrite H_eval_mem0.
+        rewrite H_eval_mem.
+        exists (get_keccak256_ctx ctx (wordToNat v') (concrete_interpreter.ConcreteInterpreter.mload' mem' v (wordToNat v'))).
+        split; reflexivity.
+        * unfold safe_sha3_cmp_ext_d in H_safe_sha3_cmp.
+          unfold safe_sha3_cmp in H_safe_sha3_cmp.
+          pose proof (H_safe_sha3_cmp d'0 H_d'0_le_d' offset size smem offset0 size0 smem0 maxidx1' sb1' maxidx2' sb2' instk_height ops H_valid_offset H_valid_size H_valid_offset0 H_valid_size0 H_valid_sb1' H_valid_sb2' H_valid_smem H_valid_smem0 H_cmp_sv1_sv2 stk mem strg ctx H_len_stk) as H_safe_sha3_cmp_0.
+
+          destruct H_safe_sha3_cmp_0 as [coffset [csize [mem1 [coffset0 [csize0 [mem2 [v [H_eval_smem [H_eval_smem0 [H_eval_offset [H_eval_size [H_eval_offset0 [H_eval_size0 [H_sha3_mem1 H_sha3_mem2]]]]]]]]]]]]]].
+
+        unfold eval_smemory in H_eval_smem.
+        destruct (map_option (EvalCommon.instantiate_memory_update (fun sv : sstack_val => eval_sstack_val sv stk mem strg ctx maxidx1' sb1' ops)) smem) as [updates|] eqn:H_eval_smem_0; try discriminate.
+        unfold eval_sstack_val in H_eval_smem_0.
+        assert (H_maxidx1_ge_S_maxidx1': S maxidx1' <= maxidx1). intuition.
+        pose proof (instantiate_memory_update_mapo_preserved_when_depth_ext_le smem (S maxidx1') maxidx1 stk mem strg ctx maxidx1' sb1' ops updates H_maxidx1_ge_S_maxidx1' H_eval_smem_0) as H_eval_smem_0_ext.
+        rewrite H_eval_smem_0_ext.
+        
+        unfold eval_smemory in H_eval_smem0.
+        destruct (map_option (EvalCommon.instantiate_memory_update (fun sv : sstack_val => eval_sstack_val sv stk mem strg ctx maxidx2' sb2' ops)) smem0) as [updates0|] eqn:H_eval_smem0_0; try discriminate.
+        unfold eval_sstack_val in H_eval_smem0_0.
+        assert (H_maxidx2_ge_S_maxidx2': S maxidx2' <= maxidx2). intuition.
+        pose proof (instantiate_memory_update_mapo_preserved_when_depth_ext_le smem0 (S maxidx2') maxidx2 stk mem strg ctx maxidx2' sb2' ops updates0 H_maxidx2_ge_S_maxidx2' H_eval_smem0_0) as H_eval_smem0_0_ext.
+        rewrite H_eval_smem0_0_ext.
+
+        unfold eval_sstack_val in H_eval_offset.
+        pose proof (eval_sstack_val'_preserved_when_depth_extended_le (S maxidx1') maxidx1 maxidx1' sb1' offset coffset stk mem strg ctx ops H_maxidx1_ge_S_maxidx1' H_eval_offset) as H_eval_offset_0.
+        rewrite H_eval_offset_0.
+
+        unfold eval_sstack_val in H_eval_size.
+        pose proof (eval_sstack_val'_preserved_when_depth_extended_le (S maxidx1') maxidx1 maxidx1' sb1' size csize stk mem strg ctx ops H_maxidx1_ge_S_maxidx1' H_eval_size) as H_eval_size_0.
+        rewrite H_eval_size_0.
+
+        unfold eval_sstack_val in H_eval_offset0.
+        pose proof (eval_sstack_val'_preserved_when_depth_extended_le (S maxidx2') maxidx2 maxidx2' sb2' offset0 coffset0 stk mem strg ctx ops H_maxidx2_ge_S_maxidx2' H_eval_offset0) as H_eval_offset0_0.
+        rewrite H_eval_offset0_0.
+
+        unfold eval_sstack_val in H_eval_size0.
+        pose proof (eval_sstack_val'_preserved_when_depth_extended_le (S maxidx2') maxidx2 maxidx2' sb2' size0 csize0 stk mem strg ctx ops H_maxidx2_ge_S_maxidx2' H_eval_size0) as H_eval_size0_0.
+        rewrite H_eval_size0_0.
+
+        injection H_eval_smem as H_eval_smem.
+        rewrite H_eval_smem.
+        injection H_eval_smem0 as H_eval_smem0.
+        rewrite H_eval_smem0.
+        
+        rewrite H_sha3_mem1.
+        rewrite H_sha3_mem2.
+        exists v.
+        split; reflexivity.          
+  Qed.
+  
 End SStackValCmpImplSoundness.
 
